If $w = f(x)$ is a differentiable function of $x$, and $x = g(t)$ is a differentiable function of $t$, then $w$ is a differentiable function of $t$, and $\frac{dw}{dt}$ can be calculated by the formula
$$
\frac{dw}{dt} = \frac{dw}{dx} \frac{dx}{dt}
$$
### Functions of Two Variable
If $w = f(x,y)$ is differentiable and if $x - x(t), y = y(t)$ are differentiable functions of $t,$ then the composition $w = f(x(t),y(t))$ is a differentiable function of $t$ and
$$
\frac{dw}{dt}=f_{x}(x(t),y(t))x'(t)+f_{y}(x(t),y(t))y'(t)
$$
or
$$
\frac{dw}{dt} =\frac{\partial f}{\partial x}\frac{dx}{dt}+\frac{\partial f}{\partial y}\frac{dy}{dt}
$$ ![[Pasted image 20240208101801.png]]

## Functions of Three Variables

If $w =f(x,y,z)$:
$$\frac{dw}{dt}= \frac{\partial w}{\partial x} \frac{dx}{dt}+\frac{\partial w}{\partial y} \frac{dy}{dt}+\frac{\partial w}{\partial z} \frac{dz}{dt}
$$
## Functions Defined on Surfaces
Consider the temperature function $w=f(x,y,z)$ at points $(x,y,z)$ on Earth's surface
$x$, $y$, and $z$ can be represented of functions of $r$ and $s$ that give the points' longitudes and latitudes.
If $x=g(r,s)$, $y=h(r,s)$, and $z=k(r,s)$ the temperature function is
$$
w = f(g(r,s),h(r,s),k(r,s))
$$
If all functions are differentiable, then $w$ has partial derivatives with respect to $r$ and $s$, given by:
$$
\begin{gather}
\frac{\partial w}{\partial r}= \frac{\partial w}{\partial x} \frac{\partial x}{\partial r}+\frac{\partial w}{\partial y} \frac{\partial y}{\partial r}+\frac{\partial w}{\partial z} \frac{\partial z}{\partial r}\\
\frac{\partial w}{\partial s}= \frac{\partial w}{\partial x} \frac{\partial x}{\partial s}+\frac{\partial w}{\partial y} \frac{\partial y}{\partial s}+\frac{\partial w}{\partial z} \frac{\partial z}{\partial s}
\end{gather}
$$
## Implicit Differentiation
Suppose that $F(x,y)$ differentiable and that the equation $F(x,y) = 0$ defines $y$ as a differentiable function of $x$. Then, at any point where $F_{y} \neq 0$:
$$
\frac{dy}{dx} = -\frac{F_{x}}{F_{y}}
$$
#### Extension to three variables:
$$
\frac{\partial z}{\partial x}=-\frac{F_{x}}{F_{y}} \text{ and }\frac{\partial z}{\partial y}=-\frac{F_{y}}{F_{z}}
$$
#### Implicit Function Theorem
[[14.4 - The Chain Rule#Extension to three variables|The above equations]] are valid if the partial derivatives $F_{x}$, $F_y$, and $F_{z}$ are continuous throughout an open region $R$ containing the point $(x_{0},y_{0},z_{0})$, and if for a constant $c$, $F(x_{0},y_{0},z_{0}) = c$ and $F_{z}(x_{0},y_{0},z_{0}) \neq 0$.
